src/HOL/IMP/Comp_Rev.thy
@@ -1,0 +1,611 @@
+theory Comp_Rev
+imports Compiler
+begin
+
+section {* Compiler Correctness, 2nd direction *}
+
+subsection {* Definitions *}
+
+text {* Execution in @{term n} steps for simpler induction *}
+primrec 
+  exec_n :: "instr list \<Rightarrow> config \<Rightarrow> nat \<Rightarrow> config \<Rightarrow> bool" 
+  ("_/ \<turnstile> (_ \<rightarrow>^_/ _)" [65,0,55,55] 55)
+where 
+  "P \<turnstile> c \<rightarrow>^0 c' = (c'=c)" |
+  "P \<turnstile> c \<rightarrow>^(Suc n) c'' = (\<exists>c'. (P \<turnstile> c \<rightarrow> c') \<and> P \<turnstile> c' \<rightarrow>^n c'')"
+
+text {* The possible successor pc's of an instruction at position @{term n} *}
+definition
+  "isuccs i n \<equiv> case i of 
+     JMP j \<Rightarrow> {n + 1 + j}
+   | JMPFLESS j \<Rightarrow> {n + 1 + j, n + 1}
+   | JMPFGE j \<Rightarrow> {n + 1 + j, n + 1}
+   | _ \<Rightarrow> {n +1}"
+
+(* FIXME: _Collect? *)
+text {* The possible successors pc's of an instruction list *}
+definition
+  "succs P n = {s. \<exists>i. 0 \<le> i \<and> i < isize P \<and> s \<in> isuccs (P!!i) (n+i)}" 
+
+text {* Possible exit pc's of a program *}
+definition
+  "exits P = succs P 0 - {0..< isize P}"
+
+  
+subsection {* Basic properties of @{term exec_n} *}
+
+lemma exec_n_exec:
+  "P \<turnstile> c \<rightarrow>^n c' \<Longrightarrow> P \<turnstile> c \<rightarrow>* c'"
+  by (induct n arbitrary: c)  (auto intro: exec.step)
+
+lemma exec_0 [intro!]: "P \<turnstile> c \<rightarrow>^0 c" by simp
+
+lemma exec_Suc [trans]:
+  "\<lbrakk> P \<turnstile> c \<rightarrow> c'; P \<turnstile> c' \<rightarrow>^n c'' \<rbrakk> \<Longrightarrow> P \<turnstile> c \<rightarrow>^Suc n c''" 
+  by (fastsimp simp del: split_paired_Ex)
+
+lemma exec_exec_n:
+  "P \<turnstile> c \<rightarrow>* c' \<Longrightarrow> \<exists>n. P \<turnstile> c \<rightarrow>^n c'"
+  by (induct rule: exec.induct) (auto intro: exec_Suc)
+    
+lemma exec_eq_exec_n:
+  "(P \<turnstile> c \<rightarrow>* c') = (\<exists>n. P \<turnstile> c \<rightarrow>^n c')"
+  by (blast intro: exec_exec_n exec_n_exec)
+
+lemma exec_n_Nil [simp]:
+  "[] \<turnstile> c \<rightarrow>^k c' = (c' = c \<and> k = 0)"
+  by (induct k) auto
+
+lemma exec1_exec_n [elim,intro!]:
+  "P \<turnstile> c \<rightarrow> c' \<Longrightarrow> P \<turnstile> c \<rightarrow>^1 c'"
+  by (cases c') simp
+
+
+subsection {* Concrete symbolic execution steps *}
+
+lemma exec_n_step:
+  "n \<noteq> n' \<Longrightarrow> 
+  P \<turnstile> (n,stk,s) \<rightarrow>^k (n',stk',s') = 
+  (\<exists>c. P \<turnstile> (n,stk,s) \<rightarrow> c \<and> P \<turnstile> c \<rightarrow>^(k - 1) (n',stk',s') \<and> 0 < k)"
+  by (cases k) auto
+
+lemma exec1_end:
+  "isize P <= fst c \<Longrightarrow> \<not> P \<turnstile> c \<rightarrow> c'"
+  by auto
+
+lemma exec_n_end:
+  "isize P <= n \<Longrightarrow> 
+  P \<turnstile> (n,s,stk) \<rightarrow>^k (n',s',stk') = (n' = n \<and> stk'=stk \<and> s'=s \<and> k =0)"
+  by (cases k) (auto simp: exec1_end)
+
+lemmas exec_n_simps = exec_n_step exec_n_end
+
+
+subsection {* Basic properties of @{term succs} *}
+
+lemma succs_simps [simp]: 
+  "succs [ADD] n = {n + 1}"
+  "succs [LOADI v] n = {n + 1}"
+  "succs [LOAD x] n = {n + 1}"
+  "succs [STORE x] n = {n + 1}"
+  "succs [JMP i] n = {n + 1 + i}"
+  "succs [JMPFGE i] n = {n + 1 + i, n + 1}"
+  "succs [JMPFLESS i] n = {n + 1 + i, n + 1}"
+  by (auto simp: succs_def isuccs_def)
+
+lemma succs_empty [iff]: "succs [] n = {}"
+  by (simp add: succs_def)
+
+lemma succs_Cons:
+  "succs (x#xs) n = isuccs x n \<union> succs xs (1+n)" (is "_ = ?x \<union> ?xs")
+proof 
+  let ?isuccs = "\<lambda>p P n i. 0 \<le> i \<and> i < isize P \<and> p \<in> isuccs (P!!i) (n+i)"
+  { fix p assume "p \<in> succs (x#xs) n"
+    then obtain i where isuccs: "?isuccs p (x#xs) n i"
+      unfolding succs_def by auto     
+    have "p \<in> ?x \<union> ?xs" 
+    proof cases
+      assume "i = 0" with isuccs show ?thesis by simp
+    next
+      assume "i \<noteq> 0" 
+      with isuccs 
+      have "?isuccs p xs (1+n) (i - 1)" by auto
+      hence "p \<in> ?xs" unfolding succs_def by blast
+      thus ?thesis .. 
+    qed
+  } 
+  thus "succs (x#xs) n \<subseteq> ?x \<union> ?xs" ..
+  
+  { fix p assume "p \<in> ?x \<or> p \<in> ?xs"
+    hence "p \<in> succs (x#xs) n"
+    proof
+      assume "p \<in> ?x" thus ?thesis by (fastsimp simp: succs_def)
+    next
+      assume "p \<in> ?xs"
+      then obtain i where "?isuccs p xs (1+n) i"
+        unfolding succs_def by auto
+      hence "?isuccs p (x#xs) n (1+i)"
+        by (simp add: algebra_simps)
+      thus ?thesis unfolding succs_def by blast
+    qed
+  }  
+  thus "?x \<union> ?xs \<subseteq> succs (x#xs) n" by blast
+qed
+
+lemma succs_iexec1:
+  "\<lbrakk> P!!i \<turnstile>i (i,s,stk) \<rightarrow> c'; 0 \<le> i; i < isize P \<rbrakk> \<Longrightarrow> fst c' \<in> succs P 0"
+  by (auto elim!: iexec1.cases simp: succs_def isuccs_def)
+
+lemma succs_shift:
+  "(p - n \<in> succs P 0) = (p \<in> succs P n)" 
+  by (fastsimp simp: succs_def isuccs_def split: instr.split)
+  
+lemma inj_op_plus [simp]:
+  "inj (op + (i::int))"
+  by (metis add_minus_cancel inj_on_inverseI)
+
+lemma succs_set_shift [simp]:
+  "op + i ` succs xs 0 = succs xs i"
+  by (force simp: succs_shift [where n=i, symmetric] intro: set_eqI)
+
+lemma succs_append [simp]:
+  "succs (xs @ ys) n = succs xs n \<union> succs ys (n + isize xs)"
+  by (induct xs arbitrary: n) (auto simp: succs_Cons algebra_simps)
+
+
+lemma exits_append [simp]:
+  "exits (xs @ ys) = exits xs \<union> (op + (isize xs)) ` exits ys - 
+                     {0..<isize xs + isize ys}" 
+  by (auto simp: exits_def image_set_diff)
+  
+lemma exits_single:
+  "exits [x] = isuccs x 0 - {0}"
+  by (auto simp: exits_def succs_def)
+  
+lemma exits_Cons:
+  "exits (x # xs) = (isuccs x 0 - {0}) \<union> (op + 1) ` exits xs - 
+                     {0..<1 + isize xs}" 
+  using exits_append [of "[x]" xs]
+  by (simp add: exits_single)
+
+lemma exits_empty [iff]: "exits [] = {}" by (simp add: exits_def)
+
+lemma exits_simps [simp]:
+  "exits [ADD] = {1}"
+  "exits [LOADI v] = {1}"
+  "exits [LOAD x] = {1}"
+  "exits [STORE x] = {1}"
+  "i \<noteq> -1 \<Longrightarrow> exits [JMP i] = {1 + i}"
+  "i \<noteq> -1 \<Longrightarrow> exits [JMPFGE i] = {1 + i, 1}"
+  "i \<noteq> -1 \<Longrightarrow> exits [JMPFLESS i] = {1 + i, 1}"
+  by (auto simp: exits_def)
+
+lemma acomp_succs [simp]:
+  "succs (acomp a) n = {n + 1 .. n + isize (acomp a)}"
+  by (induct a arbitrary: n) auto
+
+lemma acomp_size:
+  "1 \<le> isize (acomp a)"
+  by (induct a) auto
+
+lemma exits_acomp [simp]:
+  "exits (acomp a) = {isize (acomp a)}"
+  by (auto simp: exits_def acomp_size)
+
+lemma bcomp_succs:
+  "0 \<le> i \<Longrightarrow>
+  succs (bcomp b c i) n \<subseteq> {n .. n + isize (bcomp b c i)}
+                           \<union> {n + i + isize (bcomp b c i)}" 
+proof (induct b arbitrary: c i n)
+  case (And b1 b2)
+  from And.prems
+  show ?case 
+    by (cases c)
+       (auto dest: And.hyps(1) [THEN subsetD, rotated] 
+                   And.hyps(2) [THEN subsetD, rotated])
+qed auto
+
+lemmas bcomp_succsD [dest!] = bcomp_succs [THEN subsetD, rotated]
+
+lemma bcomp_exits:
+  "0 \<le> i \<Longrightarrow>
+  exits (bcomp b c i) \<subseteq> {isize (bcomp b c i), i + isize (bcomp b c i)}" 
+  by (auto simp: exits_def)
+  
+lemma bcomp_exitsD [dest!]:
+  "p \<in> exits (bcomp b c i) \<Longrightarrow> 0 \<le> i \<Longrightarrow> 
+  p = isize (bcomp b c i) \<or> p = i + isize (bcomp b c i)"
+  using bcomp_exits by auto
+
+lemma ccomp_succs:
+  "succs (ccomp c) n \<subseteq> {n..n + isize (ccomp c)}"
+proof (induct c arbitrary: n)
+  case SKIP thus ?case by simp
+next
+  case Assign thus ?case by simp
+next
+  case (Semi c1 c2)
+  from Semi.prems
+  show ?case 
+    by (fastsimp dest: Semi.hyps [THEN subsetD])
+next
+  case (If b c1 c2)
+  from If.prems
+  show ?case
+    by (auto dest!: If.hyps [THEN subsetD] simp: isuccs_def succs_Cons)
+next
+  case (While b c)
+  from While.prems
+  show ?case by (auto dest!: While.hyps [THEN subsetD])
+qed
+
+lemma ccomp_exits:
+  "exits (ccomp c) \<subseteq> {isize (ccomp c)}"
+  using ccomp_succs [of c 0] by (auto simp: exits_def)
+
+lemma ccomp_exitsD [dest!]:
+  "p \<in> exits (ccomp c) \<Longrightarrow> p = isize (ccomp c)"
+  using ccomp_exits by auto
+
+
+subsection {* Splitting up machine executions *}
+
+lemma exec1_split:
+  "P @ c @ P' \<turnstile> (isize P + i, s) \<rightarrow> (j,s') \<Longrightarrow> 0 \<le> i \<Longrightarrow> i < isize c \<Longrightarrow> 
+  c \<turnstile> (i,s) \<rightarrow> (j - isize P, s')"
+  by (auto elim!: iexec1.cases)
+
+lemma exec_n_split:
+  shows "\<lbrakk> P @ c @ P' \<turnstile> (isize P + i, s) \<rightarrow>^n (j, s');
+           0 \<le> i; i < isize c; j \<notin> {isize P ..< isize P + isize c} \<rbrakk> \<Longrightarrow>
+         \<exists>s'' i' k m. 
+                   c \<turnstile> (i, s) \<rightarrow>^k (i', s'') \<and>
+                   i' \<in> exits c \<and> 
+                   P @ c @ P' \<turnstile> (isize P + i', s'') \<rightarrow>^m (j, s') \<and>
+                   n = k + m" 
+proof (induct n arbitrary: i j s)
+  case 0
+  thus ?case by simp
+next
+  case (Suc n)
+  have i: "0 \<le> i" "i < isize c" by fact+
+  from Suc.prems
+  have j: "\<not> (isize P \<le> j \<and> j < isize P + isize c)" by simp
+  from Suc.prems 
+  obtain i0 s0 where
+    step: "P @ c @ P' \<turnstile> (isize P + i, s) \<rightarrow> (i0,s0)" and
+    rest: "P @ c @ P' \<turnstile> (i0,s0) \<rightarrow>^n (j, s')"
+    by clarsimp
+
+  from step i
+  have c: "c \<turnstile> (i,s) \<rightarrow> (i0 - isize P, s0)" by (rule exec1_split)
+
+  have "i0 = isize P + (i0 - isize P) " by simp
+  then obtain j0 where j0: "i0 = isize P + j0"  ..
+
+  note split_paired_Ex [simp del]
+
+  { assume "j0 \<in> {0 ..< isize c}"
+    with j0 j rest c
+    have ?case
+      by (fastsimp dest!: Suc.hyps intro!: exec_Suc)
+  } moreover {
+    assume "j0 \<notin> {0 ..< isize c}"
+    moreover
+    from c j0 have "j0 \<in> succs c 0"
+      by (auto dest: succs_iexec1)
+    ultimately
+    have "j0 \<in> exits c" by (simp add: exits_def)
+    with c j0 rest
+    have ?case by fastsimp
+  }
+  ultimately
+  show ?case by cases
+qed
+
+lemma exec_n_drop_right:
+  shows "\<lbrakk> c @ P' \<turnstile> (0, s) \<rightarrow>^n (j, s'); j \<notin> {0..<isize c} \<rbrakk> \<Longrightarrow>
+         \<exists>s'' i' k m. 
+                   (if c = [] then s'' = s \<and> i' = 0 \<and> k = 0
+                   else
+                   c \<turnstile> (0, s) \<rightarrow>^k (i', s'') \<and>
+                   i' \<in> exits c) \<and> 
+                   c @ P' \<turnstile> (i', s'') \<rightarrow>^m (j, s') \<and>
+                   n = k + m"
+  by (cases "c = []")
+     (auto dest: exec_n_split [where P="[]", simplified])
+  
+
+text {*
+  Dropping the left context of a potentially incomplete execution of @{term c}.
+*}
+
+lemma exec1_drop_left:
+  assumes "P1 @ P2 \<turnstile> (i, s, stk) \<rightarrow> (n, s', stk')" and "isize P1 \<le> i"
+  shows "P2 \<turnstile> (i - isize P1, s, stk) \<rightarrow> (n - isize P1, s', stk')"
+proof -
+  have "i = isize P1 + (i - isize P1)" by simp 
+  then obtain i' where "i = isize P1 + i'" ..
+  moreover
+  have "n = isize P1 + (n - isize P1)" by simp 
+  then obtain n' where "n = isize P1 + n'" ..
+  ultimately 
+  show ?thesis using assms by clarsimp
+qed
+
+lemma exec_n_drop_left:
+  "\<lbrakk> P @ P' \<turnstile> (i, s, stk) \<rightarrow>^k (n, s', stk'); 
+     isize P \<le> i; exits P' \<subseteq> {0..} \<rbrakk> \<Longrightarrow>
+     P' \<turnstile> (i - isize P, s, stk) \<rightarrow>^k (n - isize P, s', stk')"
+proof (induct k arbitrary: i s stk)
+  case 0 thus ?case by simp
+next
+  case (Suc k)
+  from Suc.prems
+  obtain i' s'' stk'' where
+    step: "P @ P' \<turnstile> (i, s, stk) \<rightarrow> (i', s'', stk'')" and
+    rest: "P @ P' \<turnstile> (i', s'', stk'') \<rightarrow>^k (n, s', stk')"
+    by auto
+  from step `isize P \<le> i`
+  have "P' \<turnstile> (i - isize P, s, stk) \<rightarrow> (i' - isize P, s'', stk'')" 
+    by (rule exec1_drop_left)
+  also
+  then have "i' - isize P \<in> succs P' 0"
+    by (fastsimp dest!: succs_iexec1)
+  with `exits P' \<subseteq> {0..}`
+  have "isize P \<le> i'" by (auto simp: exits_def)
+  from rest this `exits P' \<subseteq> {0..}`     
+  have "P' \<turnstile> (i' - isize P, s'', stk'') \<rightarrow>^k (n - isize P, s', stk')"
+    by (rule Suc.hyps)
+  finally
+  show ?case .
+qed
+
+lemmas exec_n_drop_Cons = 
+  exec_n_drop_left [where P="[instr]", simplified, standard]
+
+definition
+  "closed P \<longleftrightarrow> exits P \<subseteq> {isize P}" 
+
+lemma ccomp_closed [simp, intro!]: "closed (ccomp c)"
+  using ccomp_exits by (auto simp: closed_def)
+
+lemma acomp_closed [simp, intro!]: "closed (acomp c)"
+  by (simp add: closed_def)
+
+lemma exec_n_split_full:
+  assumes exec: "P @ P' \<turnstile> (0,s,stk) \<rightarrow>^k (j, s', stk')"
+  assumes P: "isize P \<le> j" 
+  assumes closed: "closed P"
+  assumes exits: "exits P' \<subseteq> {0..}"
+  shows "\<exists>k1 k2 s'' stk''. P \<turnstile> (0,s,stk) \<rightarrow>^k1 (isize P, s'', stk'') \<and> 
+                           P' \<turnstile> (0,s'',stk'') \<rightarrow>^k2 (j - isize P, s', stk')"
+proof (cases "P")
+  case Nil with exec
+  show ?thesis by fastsimp
+next
+  case Cons
+  hence "0 < isize P" by simp
+  with exec P closed
+  obtain k1 k2 s'' stk'' where
+    1: "P \<turnstile> (0,s,stk) \<rightarrow>^k1 (isize P, s'', stk'')" and
+    2: "P @ P' \<turnstile> (isize P,s'',stk'') \<rightarrow>^k2 (j, s', stk')"
+    by (auto dest!: exec_n_split [where P="[]" and i=0, simplified] 
+             simp: closed_def)
+  moreover
+  have "j = isize P + (j - isize P)" by simp
+  then obtain j0 where "j = isize P + j0" ..
+  ultimately
+  show ?thesis using exits
+    by (fastsimp dest: exec_n_drop_left)
+qed
+
+
+subsection {* Correctness theorem *}
+
+lemma acomp_neq_Nil [simp]:
+  "acomp a \<noteq> []"
+  by (induct a) auto
+
+lemma acomp_exec_n [dest!]:
+  "acomp a \<turnstile> (0,s,stk) \<rightarrow>^n (isize (acomp a),s',stk') \<Longrightarrow> 
+  s' = s \<and> stk' = aval a s#stk"
+proof (induct a arbitrary: n s' stk stk')
+  case (Plus a1 a2)
+  let ?sz = "isize (acomp a1) + (isize (acomp a2) + 1)"
+  from Plus.prems
+  have "acomp a1 @ acomp a2 @ [ADD] \<turnstile> (0,s,stk) \<rightarrow>^n (?sz, s', stk')" 
+    by (simp add: algebra_simps)
+      
+  then obtain n1 s1 stk1 n2 s2 stk2 n3 where 
+    "acomp a1 \<turnstile> (0,s,stk) \<rightarrow>^n1 (isize (acomp a1), s1, stk1)"
+    "acomp a2 \<turnstile> (0,s1,stk1) \<rightarrow>^n2 (isize (acomp a2), s2, stk2)" 
+       "[ADD] \<turnstile> (0,s2,stk2) \<rightarrow>^n3 (1, s', stk')"
+    by (auto dest!: exec_n_split_full)
+
+  thus ?case by (fastsimp dest: Plus.hyps simp: exec_n_simps)
+qed (auto simp: exec_n_simps)
+
+lemma bcomp_split:
+  shows "\<lbrakk> bcomp b c i @ P' \<turnstile> (0, s, stk) \<rightarrow>^n (j, s', stk'); 
+           j \<notin> {0..<isize (bcomp b c i)}; 0 \<le> i \<rbrakk> \<Longrightarrow>
+         \<exists>s'' stk'' i' k m. 
+           bcomp b c i \<turnstile> (0, s, stk) \<rightarrow>^k (i', s'', stk'') \<and>
+           (i' = isize (bcomp b c i) \<or> i' = i + isize (bcomp b c i)) \<and>
+           bcomp b c i @ P' \<turnstile> (i', s'', stk'') \<rightarrow>^m (j, s', stk') \<and>
+           n = k + m"
+  by (cases "bcomp b c i = []")
+     (fastsimp dest!: exec_n_drop_right)+
+
+lemma bcomp_exec_n [dest]:
+  "\<lbrakk> bcomp b c j \<turnstile> (0, s, stk) \<rightarrow>^n (i, s', stk');
+     isize (bcomp b c j) \<le> i; 0 \<le> j \<rbrakk> \<Longrightarrow>
+  i = isize(bcomp b c j) + (if c = bval b s then j else 0) \<and>
+  s' = s \<and> stk' = stk"
+proof (induct b arbitrary: c j i n s' stk')
+  case B thus ?case 
+    by (simp split: split_if_asm add: exec_n_simps)
+next
+  case (Not b) 
+  from Not.prems show ?case
+    by (fastsimp dest!: Not.hyps) 
+next
+  case (And b1 b2)
+  
+  let ?b2 = "bcomp b2 c j" 
+  let ?m  = "if c then isize ?b2 else isize ?b2 + j"
+  let ?b1 = "bcomp b1 False ?m" 
+
+  have j: "isize (bcomp (And b1 b2) c j) \<le> i" "0 \<le> j" by fact+
+  
+  from And.prems
+  obtain s'' stk'' i' k m where 
+    b1: "?b1 \<turnstile> (0, s, stk) \<rightarrow>^k (i', s'', stk'')"
+        "i' = isize ?b1 \<or> i' = ?m + isize ?b1" and
+    b2: "?b2 \<turnstile> (i' - isize ?b1, s'', stk'') \<rightarrow>^m (i - isize ?b1, s', stk')"
+    by (auto dest!: bcomp_split dest: exec_n_drop_left)
+  from b1 j
+  have "i' = isize ?b1 + (if \<not>bval b1 s then ?m else 0) \<and> s'' = s \<and> stk'' = stk"
+    by (auto dest!: And.hyps)
+  with b2 j
+  show ?case 
+    by (fastsimp dest!: And.hyps simp: exec_n_end split: split_if_asm)
+next
+  case Less
+  thus ?case by (auto dest!: exec_n_split_full simp: exec_n_simps) (* takes time *) 
+qed
+
+lemma ccomp_empty [elim!]:
+  "ccomp c = [] \<Longrightarrow> (c,s) \<Rightarrow> s"
+  by (induct c) auto
+
+lemma assign [simp]:
+  "(x ::= a,s) \<Rightarrow> s' \<longleftrightarrow> (s' = s(x := aval a s))"
+  by auto
+
+lemma ccomp_exec_n:
+  "ccomp c \<turnstile> (0,s,stk) \<rightarrow>^n (isize(ccomp c),t,stk')
+  \<Longrightarrow> (c,s) \<Rightarrow> t \<and> stk'=stk"
+proof (induct c arbitrary: s t stk stk' n)
+  case SKIP
+  thus ?case by auto
+next
+  case (Assign x a)
+  thus ?case
+    by simp (fastsimp dest!: exec_n_split_full simp: exec_n_simps)
+next
+  case (Semi c1 c2)
+  thus ?case by (fastsimp dest!: exec_n_split_full)
+next
+  case (If b c1 c2)
+  note If.hyps [dest!]
+
+  let ?if = "IF b THEN c1 ELSE c2"
+  let ?cs = "ccomp ?if"
+  let ?bcomp = "bcomp b False (isize (ccomp c1) + 1)"
+  
+  from `?cs \<turnstile> (0,s,stk) \<rightarrow>^n (isize ?cs,t,stk')`
+  obtain i' k m s'' stk'' where
+    cs: "?cs \<turnstile> (i',s'',stk'') \<rightarrow>^m (isize ?cs,t,stk')" and
+        "?bcomp \<turnstile> (0,s,stk) \<rightarrow>^k (i', s'', stk'')" 
+        "i' = isize ?bcomp \<or> i' = isize ?bcomp + isize (ccomp c1) + 1"
+    by (auto dest!: bcomp_split)
+
+  hence i':
+    "s''=s" "stk'' = stk" 
+    "i' = (if bval b s then isize ?bcomp else isize ?bcomp+isize(ccomp c1)+1)"
+    by auto
+  
+  with cs have cs':
+    "ccomp c1@JMP (isize (ccomp c2))#ccomp c2 \<turnstile> 
+       (if bval b s then 0 else isize (ccomp c1)+1, s, stk) \<rightarrow>^m
+       (1 + isize (ccomp c1) + isize (ccomp c2), t, stk')"
+    by (fastsimp dest: exec_n_drop_left simp: exits_Cons isuccs_def algebra_simps)
+     
+  show ?case
+  proof (cases "bval b s")
+    case True with cs'
+    show ?thesis
+      by simp
+         (fastsimp dest: exec_n_drop_right 
+                   split: split_if_asm simp: exec_n_simps)
+  next
+    case False with cs'
+    show ?thesis
+      by (auto dest!: exec_n_drop_Cons exec_n_drop_left 
+               simp: exits_Cons isuccs_def)
+  qed
+next
+  case (While b c)
+
+  from While.prems
+  show ?case
+  proof (induct n arbitrary: s rule: nat_less_induct)
+    case (1 n)
+    
+    { assume "\<not> bval b s"
+      with "1.prems"
+      have ?case
+        by simp
+           (fastsimp dest!: bcomp_exec_n bcomp_split 
+                     simp: exec_n_simps)
+    } moreover {
+      assume b: "bval b s"
+      let ?c0 = "WHILE b DO c"
+      let ?cs = "ccomp ?c0"
+      let ?bs = "bcomp b False (isize (ccomp c) + 1)"
+      let ?jmp = "[JMPB (isize ?bs + isize (ccomp c) + 1)]"
+      
+      from "1.prems" b
+      obtain k where
+        cs: "?cs \<turnstile> (isize ?bs, s, stk) \<rightarrow>^k (isize ?cs, t, stk')" and
+        k:  "k \<le> n"
+        by (fastsimp dest!: bcomp_split)
+      
+      have ?case
+      proof cases
+        assume "ccomp c = []"
+        with cs k
+        obtain m where
+          "?cs \<turnstile> (0,s,stk) \<rightarrow>^m (isize (ccomp ?c0), t, stk')"
+          "m < n"
+          by (auto simp: exec_n_step [where k=k])
+        with "1.hyps"
+        show ?case by blast
+      next
+        assume "ccomp c \<noteq> []"
+        with cs
+        obtain m m' s'' stk'' where
+          c: "ccomp c \<turnstile> (0, s, stk) \<rightarrow>^m' (isize (ccomp c), s'', stk'')" and 
+          rest: "?cs \<turnstile> (isize ?bs + isize (ccomp c), s'', stk'') \<rightarrow>^m 
+                       (isize ?cs, t, stk')" and
+          m: "k = m + m'"
+          by (auto dest: exec_n_split [where i=0, simplified])
+        from c
+        have "(c,s) \<Rightarrow> s''" and stk: "stk'' = stk"
+          by (auto dest!: While.hyps)
+        moreover
+        from rest m k stk
+        obtain k' where
+          "?cs \<turnstile> (0, s'', stk) \<rightarrow>^k' (isize ?cs, t, stk')"
+          "k' < n"
+          by (auto simp: exec_n_step [where k=m])
+        with "1.hyps"
+        have "(?c0, s'') \<Rightarrow> t \<and> stk' = stk" by blast
+        ultimately
+        show ?case using b by blast
+      qed
+    }
+    ultimately show ?case by cases
+  qed
+qed
+
+theorem ccomp_exec:
+  "ccomp c \<turnstile> (0,s,stk) \<rightarrow>* (isize(ccomp c),t,stk') \<Longrightarrow> (c,s) \<Rightarrow> t"
+  by (auto dest: exec_exec_n ccomp_exec_n)
+
+corollary ccomp_sound:
+  "ccomp c \<turnstile> (0,s,stk) \<rightarrow>* (isize(ccomp c),t,stk)  \<longleftrightarrow>  (c,s) \<Rightarrow> t"
+  by (blast intro!: ccomp_exec ccomp_bigstep)
+
+end
